afi definition & free_in_context lemma
See sf StlcProp.v

src/Coq/Syntax.v
@@ -164,6 +164,39 @@ Inductive subst_list : Exp -> [Var] -> [Exp] -> Exp -> Prop :=
     [;es \ vs;] e2 = e3 ->
     [; e'::es \ v::vs ;] e1 = e3
 where " [; es '\' vs ;] e1 '=' e2 " := (subst_list e1 vs es e2).
+Print ExpVar.
+
+Inductive appears_free_in : Var -> Exp -> Prop :=
+  | afi_var : forall x,
+    appears_free_in x (ExpVar x)
+  | afi_field : forall x e fi,
+    appears_free_in x e ->
+    appears_free_in x (ExpFieldAccess e fi)
+  | afi_m_invk1 : forall x e mname es,
+    appears_free_in x e ->
+    appears_free_in x (ExpMethodInvoc e mname es)
+  | afi_m_invk2 : forall x e e' mname es,
+    In e' es ->
+    appears_free_in x e' ->
+    appears_free_in x (ExpMethodInvoc e mname es)
+  | afi_cast : forall x e CName,
+    appears_free_in x e ->
+    appears_free_in x (ExpCast CName e)
+  | afi_new : forall x e es CName,
+    In e es ->
+    appears_free_in x e ->
+    appears_free_in x (ExpNew CName es).
+
+Hint Constructors appears_free_in.
+Tactic Notation "afi_cases" tactic(first) ident(c) :=
+  first;
+  [ Case_aux c "afi_var" | Case_aux c "afi_field"
+  | Case_aux c "afi_m_invk1" | Case_aux c "afi_m_invk2"
+  | Case_aux c "afi_cast" | Case_aux c "afi_new"].
+
+
+Definition closed (e: Exp) :=
+  forall x, ~ appears_free_in x e.
 
 Inductive Warning (s: string) : Prop :=
   | w_str : Warning s.
